deterministic type kinding and elaboration
Implements Professor Xie's suggestion of requiring kind annotations on
empty rows. This makes type kinding and elaboration deterministic, which
will make many future proofs easier.

TabularTypeInterpreter/F⊗⊕ω/Lemmas/Type.lean
@@ -1,3 +1,4 @@
+import Aesop
 import TabularTypeInterpreter.«F⊗⊕ω».Semantics.Environment
 import TabularTypeInterpreter.«F⊗⊕ω».Semantics.Type
 
@@ -210,6 +211,31 @@ theorem TypeVar_open_eq {A : «Type»} (Alc : A.TypeVarLocallyClosed n) : A.Type
   | .sum .. => let .sum A'lc := Alc; rw [TypeVar_open, A'lc.TypeVar_open_eq]
 
 end TypeVarLocallyClosed
+
+@[elab_as_elim]
+def rec_uniform {motive : «Type» → Prop} (var : ∀ a : TypeVar, motive (var a))
+  (lam : ∀ K A, motive A → motive (lam K A)) (app : ∀ A B, motive A → motive B → motive (app A B))
+  («forall» : ∀ K A, motive A → motive («forall» K A))
+  (arr : ∀ A B, motive A → motive B → motive (arr A B))
+  (list : ∀ As, (∀ A ∈ As, motive A) → motive (list As))
+  (listApp : ∀ A B, motive A → motive B → motive (listApp A B))
+  (prod : ∀ A, motive A → motive (prod A)) (sum : ∀ A, motive A → motive (sum A)) (A : «Type»)
+  : motive A :=
+  rec (motive_1 := motive) var lam app «forall» arr list listApp prod sum (fun _ => (nomatch ·))
+    (fun _ _ ih₀ ih₁ _ mem => match mem with | .head _ => ih₀ | .tail _ mem' => ih₁ _ mem') A
+
+theorem TypeVar_open_not_mem_freeTypeVars_preservation_of_ne
+  : a ≠ a' → a ∉ freeTypeVars A → a ∉ (A.TypeVar_open a' n).freeTypeVars := by
+  induction A using rec_uniform generalizing n <;> aesop
+    (add simp [TypeVar_open, freeTypeVars], safe cases TypeVar)
+
+set_option maxHeartbeats 2000000 in
+theorem TypeVar_open_inj_of_not_mem_freeTypeVars (aninA : a ∉ freeTypeVars A)
+  (aninB : a ∉ freeTypeVars B) (eq : A.TypeVar_open a n = B.TypeVar_open a n) : A = B := by
+  induction A using rec_uniform generalizing B n <;>
+    induction B using rec_uniform <;> aesop
+    (add simp [TypeVar_open, freeTypeVars], safe cases TypeVar,
+      10% apply List.eq_of_map_eq_map_of_inj)
 
 end «Type»
 
