TabularTypeInterpreter/Lemmas/TypeEnvironment.lean
@@ -1,7 +1,9 @@
 import TabularTypeInterpreter.Semantics.Type.KindingAndElaboration
 import TabularTypeInterpreter.Theorems.Kind
 
-namespace TabularTypeInterpreter.TypeEnvironment.WellFormednessAndElaboration
+namespace TabularTypeInterpreter.TypeEnvironment
+
+namespace WellFormednessAndElaboration
 
 theorem TypeVarIn_preservation (Γwe : [[Γc ⊢ Γ ⇝ Δ]])
   (aκinΓ : [[a : κ ∈ Γ]]) (κe : [[⊢ κ ⇝ K]]) : [[a : K ∈ Δ]] :=
@@ -28,4 +30,28 @@ theorem TermVarNotInDom_preservation (Γwe : [[Γc ⊢ Γ ⇝ Δ]]) (xnin : [[x 
     | .inl (.refl _) => xnin <| .head _
     | .inr xinΔ' => Γ'we.TermVarNotInDom_preservation (List.not_mem_of_not_mem_cons xnin) xinΔ'
 
-end TabularTypeInterpreter.TypeEnvironment.WellFormednessAndElaboration
+end WellFormednessAndElaboration
+
+theorem TypeVarIn.deterministic (aκ₀in : [[a : κ₀ ∈ Γ]]) (aκ₁in : [[a : κ₁ ∈ Γ]])
+  : κ₀ = κ₁ := match Γ with
+  | .empty => nomatch aκ₀in
+  | .typeExt .. => by
+    cases aκ₀in
+    · case head =>
+      cases aκ₁in
+      · case head => rfl
+      · case typeExt => contradiction
+    · case typeExt aκ₀in' _ =>
+      cases aκ₁in
+      · case head => contradiction
+      · case typeExt aκ₁in' _ => exact aκ₀in'.deterministic aκ₁in'
+  | .termExt .. =>
+    let .termExt aκ₀in' := aκ₀in
+    let .termExt aκ₁in' := aκ₁in
+    aκ₀in'.deterministic aκ₁in'
+  | .constrExt .. =>
+    let .constrExt aκ₀in' := aκ₀in
+    let .constrExt aκ₁in' := aκ₁in
+    aκ₀in'.deterministic aκ₁in'
+
+end TabularTypeInterpreter.TypeEnvironment
